Function call framework - only floyd condition left

Steps.thy
@@ -2,27 +2,22 @@ theory Steps
   imports Blocks
 begin
 
-
 context fixes program :: "llvm_program"
 begin
 
+section "Step Relation"
 
-datatype instruction_state = execi "llvm_identifier option" llvm_instruction_block state
+datatype instruction_state = 
+    execi "llvm_identifier option" llvm_instruction_block state
   | flowi state llvm_block_return
   | is_erri: erri
 
-datatype (discs_sels) function_state = branchf (state: state) "llvm_identifier option" llvm_identifier llvm_identifier
-  | retf (state: state) (ret_value: "llvm_value option")
+datatype (discs_sels) function_state = 
+    branchf (state: state) "llvm_identifier option" llvm_identifier llvm_identifier
+  | retf (state: state) (ret_value: "llvm_value option") (ret_func: llvm_identifier)
   | is_errf: errf
 
-
 definition "first_label f \<equiv> (case llvm_function.blocks f of ((l,b)#fs) \<Rightarrow> Some l | _ \<Rightarrow> None)"
-
-
-
-
-
-
 
 inductive
   step_i :: "instruction_state \<Rightarrow> instruction_state \<Rightarrow> bool" (infix "\<rightarrow>\<^sub>i" 50)
@@ -47,7 +42,7 @@ where
 (* Function calls *)
 | "map_of (funcs program) f = Some fu
   \<Longrightarrow> first_label fu = Some b
-  \<Longrightarrow> step_f\<^sup>*\<^sup>* (branchf (push_frame s) None b f) (retf s' v')
+  \<Longrightarrow> step_f\<^sup>*\<^sup>* (branchf (push_frame s) None b f) (retf s' v' f)
   \<Longrightarrow> (execi pre ([],(call n ty f p)#is,t) s) \<rightarrow>\<^sub>i (execi pre ([],is,t) (pop_frame s s'))"
 | "map_of (funcs program) f = None
   \<Longrightarrow> (execi pre ([],(call n ty f p)#is,t) s) \<rightarrow>\<^sub>i erri"
@@ -81,7 +76,7 @@ where
 | "map_of (funcs program) f = Some fu \<Longrightarrow>
     map_of (llvm_function.blocks fu) lab = Some b \<Longrightarrow>
     step_i\<^sup>*\<^sup>* (execi prev b s) (flowi s' (return_value v)) \<Longrightarrow>
-    branchf s prev lab f \<rightarrow>\<^sub>f retf s' v"
+    branchf s prev lab f \<rightarrow>\<^sub>f retf s' v f"
 
 (* Block errors *)
 | "map_of (funcs program) f = Some fu \<Longrightarrow>
@@ -95,213 +90,18 @@ where
      branchf s prev lab f \<rightarrow>\<^sub>f errf"
 
 
-inductive trans_closure_n where
-  "trans_closure_n R s n s"
-| "trans_closure_n R s' m s'' \<Longrightarrow> R s n s' \<Longrightarrow> trans_closure_n R s (m+n) s''"
-
-lemma trans_closure_n_mono [mono]:
-  assumes "(\<And>s n s'. A s n s' \<longrightarrow> B s n s')"
-  shows "trans_closure_n A s n s' \<longrightarrow> trans_closure_n B s n s'" 
-  apply (rule impI)
-  using assms apply -
-  by (induction rule: trans_closure_n.induct; simp add: trans_closure_n.intros)
-
-
-inductive
-  step_i_n :: "instruction_state \<Rightarrow> nat \<Rightarrow> instruction_state \<Rightarrow> bool"
-and
-  step_f_n :: "function_state \<Rightarrow> nat \<Rightarrow> function_state \<Rightarrow> bool"
-where
-(* Control flow *)
-"step_i_n (execi pre ([],[],br_label l) s) n (flowi s (branch_label l))"
-
-| "dereference s b = ok (vi1 b') \<Longrightarrow>
-    step_i_n (execi pre ([],[],br_i1 b l1 l2) s) n (flowi s (branch_label (if b' then l1 else l2)))"
-| "\<nexists>b'. dereference s b = ok (vi1 b') \<Longrightarrow>
-    step_i_n (execi pre ([],[],br_i1 b l1 l2) s) n erri"
-
-| "step_i_n (execi pre ([],[],ret None) s) n (flowi s (return_value None))"
-
-| "dereference s v = ok v' \<Longrightarrow>
-    step_i_n (execi pre ([],[],ret (Some (t, v))) s) n (flowi s (return_value (Some v')))"
-| "dereference s v = err _ \<Longrightarrow>
-    step_i_n (execi pre ([],[],ret (Some (t, v))) s) n erri"
-
-
-(* Function calls *)
-| "map_of (funcs program) f = Some fu
-  \<Longrightarrow> first_label fu = Some b
-  \<Longrightarrow> trans_closure_n (step_f_n) (branchf (push_frame s) None b f) n (retf s' v')
-  \<Longrightarrow> step_i_n (execi pre ([],(call na ty f p)#is,t) s) (n+1) (execi pre ([],is,t) (pop_frame s s'))"
-
-| "map_of (funcs program) f = None
-  \<Longrightarrow> step_i_n (execi pre ([],(call na ty f p)#is,t) s) n erri"
-| "map_of (funcs program) f = Some fu
-  \<Longrightarrow> first_label fu = None
-  \<Longrightarrow> step_i_n (execi pre ([],(call na ty f p)#is,t) s) n erri"
-
-| "map_of (funcs program) f = Some fu
-  \<Longrightarrow> first_label fu = Some b
-  \<Longrightarrow> trans_closure_n (step_f_n) (branchf (push_frame s) None b f) n errf
-  \<Longrightarrow> step_i_n (execi pre ([],(call na ty f p)#is,t) s) (n+1) erri"
-
-
-(* Normal instructions *)
-| "execute_instruction i s = ok s'
-  \<Longrightarrow> \<not>is_call i
-  \<Longrightarrow> step_i_n (execi pre ([],i#is,t) s) n (execi pre ([],is,t) s')"
-| "execute_instruction i s = err _
-  \<Longrightarrow> \<not>is_call i
-  \<Longrightarrow> step_i_n (execi pre ([],i#is,t) s) n erri"
-
-
-(* Phi nodes *)
-| "execute_phi pre p s = ok s' \<Longrightarrow>
-    step_i_n (execi pre (p#ps,is,t) s) n (execi pre (ps,is,t) s')"
-| "execute_phi pre p s = err _ \<Longrightarrow>
-    step_i_n (execi pre (p#ps,is,t) s) n erri"
-
-
-(* Blocks *)
-| "map_of (funcs program) f = Some fu \<Longrightarrow>
-    map_of (llvm_function.blocks fu) lab = Some b \<Longrightarrow>
-    trans_closure_n (step_i_n) (execi prev b s) n (flowi s' (branch_label l)) \<Longrightarrow>                                                          
-    step_f_n (branchf s prev lab f) n (branchf s' (Some lab) l f)"
-| "map_of (funcs program) f = Some fu \<Longrightarrow>
-    map_of (llvm_function.blocks fu) lab = Some b \<Longrightarrow>
-    trans_closure_n (step_i_n) (execi prev b s) n (flowi s' (return_value v)) \<Longrightarrow>
-    step_f_n (branchf s prev lab f) n (retf s' v)"
-
-
-(* Block errors *)
-| "map_of (funcs program) f = Some fu \<Longrightarrow>
-    map_of (llvm_function.blocks fu) lab = Some b \<Longrightarrow>
-    trans_closure_n (step_i_n) (execi prev b s) n erri \<Longrightarrow>
-    step_f_n (branchf s prev lab f) n errf"
-| "map_of (funcs program) f = Some fu \<Longrightarrow>
-    map_of (llvm_function.blocks fu) lab = None \<Longrightarrow>
-     step_f_n (branchf s prev lab f) n errf"
-| "map_of (funcs program) f = None \<Longrightarrow>
-     step_f_n (branchf s prev lab f) n errf"
-
-
-
-lemma rtranclp_impl_exists_trans_closure_n:
-  assumes "R\<^sup>*\<^sup>* s s'"
-  assumes "(\<And>s s'. R s s' \<Longrightarrow> \<exists>n. R' s n s')"
-  shows "\<exists>n. trans_closure_n R' s n s'"
-  using assms trans_closure_n.intros
-  by (induction rule: converse_rtranclp_induct, force, fastforce)
-
-lemma trans_closure_n_impl_rtranclp:
-  assumes "trans_closure_n R' s n s'"
-  assumes "(\<And>s s' n. R' s n s' \<Longrightarrow> R s s')"
-  shows "R\<^sup>*\<^sup>* s s'"
-  using assms trans_closure_n.intros converse_rtranclp_into_rtranclp
-  by (induction rule: trans_closure_n.induct, blast, smt)
-
-
-lemma n_step_impl_step:
-  "step_i_n si n si' \<Longrightarrow> step_i si si'"
-  "step_f_n sf n sf' \<Longrightarrow> step_f sf sf'"
-   apply (induction rule: step_i_n_step_f_n.inducts)
-  using step_i_step_f.intros trans_closure_n_impl_rtranclp
-  by (metis (no_types, lifting))+
-
-lemma step_impl_exists_n_step:
-  "step_i si si' \<Longrightarrow> \<exists>n. step_i_n si n si'"
-  "step_f sf sf' \<Longrightarrow> \<exists>n. step_f_n sf n sf'"
-  apply (induction rule: step_i_step_f.inducts)
-  apply (simp add: step_i_n_step_f_n.intros)+
-  subgoal premises prems for f fu b s s' v' pre n ty p ins t
-  proof -
-    obtain n where "trans_closure_n (step_f_n) (branchf (push_frame s) None b f) n (retf s' v')"
-      using prems(3)
-      apply (induction rule: converse_rtranclp_induct)
-      apply (simp add: trans_closure_n.intros(1))
-      by (meson trans_closure_n.intros(2))
-
-    then show ?thesis
-      using prems step_i_n_step_f_n.intros(7)
-      by blast
-  qed
-  apply (simp add: step_i_n_step_f_n.intros)+
-  subgoal premises prems for f fu b s pre n ty p ins t
-  proof -
-    obtain n where "trans_closure_n (step_f_n) (branchf (push_frame s) None b f) n errf"
-      using prems(3)
-      apply (induction rule: converse_rtranclp_induct)
-      apply (simp add: trans_closure_n.intros(1))
-      by (meson trans_closure_n.intros(2))
-
-    then show ?thesis
-      using prems step_i_n_step_f_n.intros(10)
-      by blast
-  qed
-  apply (simp add: step_i_n_step_f_n.intros)+
-  subgoal premises prems for f fu lab b prev s s' l
-  proof -
-    obtain n where "trans_closure_n (step_i_n) (execi prev b s) n (flowi s' (branch_label l))"
-      using prems(3)
-      apply (induction rule: converse_rtranclp_induct)
-      apply (simp add: trans_closure_n.intros(1))
-      by (meson trans_closure_n.intros(2))
-
-    then show ?thesis
-      using prems step_i_n_step_f_n.intros(15)
-      by blast
-  qed
-  subgoal premises prems for f fu lab b prev s s' v
-  proof -
-    obtain n where "trans_closure_n (step_i_n) (execi prev b s) n (flowi s' (return_value v))"
-      using prems(3)
-      apply (induction rule: converse_rtranclp_induct)
-      apply (simp add: trans_closure_n.intros(1))
-      by (meson trans_closure_n.intros(2))
-
-    then show ?thesis
-      using prems step_i_n_step_f_n.intros(16)
-      by blast
-  qed
-  subgoal premises prems for f fu lab b prev s
-  proof -
-    obtain n where "trans_closure_n (step_i_n) (execi prev b s) n erri"
-      using prems(3)
-      apply (induction rule: converse_rtranclp_induct)
-      apply (simp add: trans_closure_n.intros(1))
-      by (meson trans_closure_n.intros(2))
-
-    then show ?thesis
-      using prems step_i_n_step_f_n.intros(17)
-      by blast
-  qed
-  by (simp add: step_i_n_step_f_n.intros)+
-
-lemma steps_impl_exists_n_steps:
-  "step_i\<^sup>*\<^sup>* si si' \<Longrightarrow> \<exists>n. trans_closure_n (step_i_n) si n si'"
-  "step_f\<^sup>*\<^sup>* sf sf' \<Longrightarrow> \<exists>n. trans_closure_n (step_f_n) sf n sf'"
-  using rtranclp_impl_exists_trans_closure_n step_impl_exists_n_step
-  by metis+
-
-lemma n_steps_impl_steps:
-  "trans_closure_n (step_i_n) si n si' \<Longrightarrow> step_i\<^sup>*\<^sup>* si si'"
-  "trans_closure_n (step_f_n) sf n sf' \<Longrightarrow> step_f\<^sup>*\<^sup>* sf sf'"
-  using n_step_impl_step trans_closure_n_impl_rtranclp
-  by metis+
-
-
 abbreviation steps_i (infix "\<rightarrow>\<^sub>i*" 50) where
   "s \<rightarrow>\<^sub>i* s' \<equiv> step_i\<^sup>*\<^sup>* s s'"
 abbreviation steps_f :: "function_state \<Rightarrow> function_state \<Rightarrow> bool" (infix "\<rightarrow>\<^sub>f*" 50) where
   "s \<rightarrow>\<^sub>f* s' \<equiv> step_f\<^sup>*\<^sup>* s s'"
 
 
-
+section "Terminal States"
 
 definition terminal_i where
   "terminal_i s \<equiv> (case s of flowi _ _ \<Rightarrow> True | erri \<Rightarrow> True | _ \<Rightarrow> False)"
 definition terminal_f where
-  "terminal_f s \<equiv> (case s of retf _ _ \<Rightarrow> True | errf \<Rightarrow> True | _ \<Rightarrow> False)"
+  "terminal_f s \<equiv> (case s of retf _ _ _ \<Rightarrow> True | errf \<Rightarrow> True | _ \<Rightarrow> False)"
 
 notation terminal_i ("_ \<nexists>\<rightarrow>\<^sub>i" 50)
 notation terminal_f ("_ \<nexists>\<rightarrow>\<^sub>f" 50)
@@ -316,11 +116,10 @@ lemma terminal_state_simps[simp]:
   "erri \<nexists>\<rightarrow>\<^sub>i"
   "\<not>(execi pre b s \<nexists>\<rightarrow>\<^sub>i)"
   "errf \<nexists>\<rightarrow>\<^sub>f"
-  "retf s v \<nexists>\<rightarrow>\<^sub>f"
+  "retf s v f \<nexists>\<rightarrow>\<^sub>f"
   "\<not>(branchf s p l f \<nexists>\<rightarrow>\<^sub>f)"
   unfolding terminal_i_def terminal_f_def
   by auto
-
 
 lemma terminates_impl_exists_next_state:
   "terminates_to_i si si' \<Longrightarrow> \<not>terminal_i si \<Longrightarrow> \<exists>si'. si \<rightarrow>\<^sub>i si'"
@@ -345,6 +144,9 @@ lemma terminal_steps_refl[simp]:
   apply (auto elim: converse_rtranclpE; metis converse_rtranclpE terminal_impl_no_next_state(2))
   done
 
+
+section "Determinism"
+
 lemma step_deterministic[simp]:
   "si \<rightarrow>\<^sub>i si' \<Longrightarrow> \<forall>s'. si \<rightarrow>\<^sub>i s' \<longrightarrow> s' = si'"
   "sf \<rightarrow>\<^sub>f sf' \<Longrightarrow> \<forall>s'. sf \<rightarrow>\<^sub>f s' \<longrightarrow> s' = sf'"
@@ -357,10 +159,10 @@ lemma step_deterministic[simp]:
   using step_i.simps apply fastforce
   subgoal premises prems for f fu b s s' v' pre na ty p ins t
   proof -
-    have "branchf (push_frame s) None b f \<rightarrow>\<^sub>f* retf s' v'"
+    have "branchf (push_frame s) None b f \<rightarrow>\<^sub>f* retf s' v' f"
       by (metis (no_types, lifting) mono_rtranclp prems(3))
 
-    then have "\<And>s'' v''. branchf (push_frame s) None b f \<rightarrow>\<^sub>f* retf s'' v'' \<longrightarrow> (s'' = s' \<and> v'' = v')"
+    then have "\<And>s'' v'' f'. branchf (push_frame s) None b f \<rightarrow>\<^sub>f* retf s'' v'' f' \<longrightarrow> (s'' = s' \<and> v'' = v' \<and> f' = f)"
       using prems(3) 
       apply (induction rule: converse_rtranclp_induct)
       apply (metis function_state.inject(2) terminal_impl_no_next_state(2) converse_rtranclpE terminal_state_simps(5))
@@ -388,7 +190,7 @@ lemma step_deterministic[simp]:
 
     moreover
 
-    have "\<And>s' v'. \<not>(branchf (push_frame s) None b f) \<rightarrow>\<^sub>f* retf s' v'"
+    have "\<And>s' v'. \<not>(branchf (push_frame s) None b f) \<rightarrow>\<^sub>f* retf s' v' f"
       using prems(3)
       apply (induction rule: converse_rtranclp_induct)
       apply (metis terminal_impl_no_next_state(2) terminal_state_simps(4) converse_rtranclpE function_state.distinct(5))
@@ -475,166 +277,29 @@ lemma step_deterministic[simp]:
 
 
 
-
-
-
-
-
-
-
-
-
-
-
-
-
-
-
+section "Weakest Precondition over Steps"
 
 definition "wp_steps_i s Q \<equiv> \<forall>s'. terminates_to_i s s' \<longrightarrow> \<not>is_erri s' \<and> Q s'"
-
 definition "wp_steps_f_post s p s' Q \<equiv> (\<not>is_errf s') \<and> (Q (state s) p (state s') (ret_value s'))"
 definition "wp_steps_f s p Q \<equiv> \<forall>s'. terminates_to_f s s' \<longrightarrow> wp_steps_f_post s p s' Q"
 
 
 
-
-
-
-
-
-section "Instruction Step Intro Rules"
-
-named_theorems wp_instrs_intro
-(*
-lemma instrs_phi_intro[wp_instrs_intro]:
-  assumes "wp (execute_phi pre p s) (\<lambda>s'. wp_instrs (execi pre (ps, is, t) s') Q)"
-  shows "wp_instrs (execi pre (p#ps, is, t) s) Q"
-proof -
-  obtain s' where nextstate: "execute_phi pre p s = ok s'"
-    using assms wp_impl_ok
-    by blast
-
-  show ?thesis
-    using nextstate assms converse_rtranclpE fst_conv instruction_state.sel list.discI Steps.step_deterministic
-      list.inject result.distinct result.simps snd_conv step_i.cases terminal_state_simps local.step_i_step_f.intros
-      result.inject(1)
-    unfolding wp_gen_def wp_instrs_def terminal_i_def
-    by (smt (verit, del_insts))
-qed
-
-lemma instrs_instr_intro[wp_instrs_intro]:
-  assumes "\<not>is_call i"
-  assumes "wp (execute_instruction i s) (\<lambda>s'. wp_instrs (execi pre ([], is, t) s') Q)"
-  shows "wp_instrs (execi pre ([], i#is, t) s) Q"
-proof -
-  obtain s' where nextstate: "execute_instruction i s = ok s'"
-    using assms wp_impl_ok
-    by blast
-
-  show ?thesis
-    using nextstate assms converse_rtranclpE fst_conv instruction_state.sel list.discI Steps.step_deterministic
-      list.inject result.distinct result.simps snd_conv step_i.cases terminal_state_simps local.step_i_step_f.intros
-      result.inject(1)
-    unfolding wp_gen_def wp_instrs_def terminal_i_def
-    by (smt (verit, del_insts))
-qed
-
-lemma block_ret_Some_wp_intro[wp_instrs_intro]:
-  assumes "register_\<alpha> s value = Some v"
-  assumes "Q (flowi s (return_value (Some v)))"
-  shows "wp_instrs (execi pre ([], [], ret (Some (type, value))) s) Q"
-  unfolding wp_instrs_def
-  using assms
-  apply (intro impI allI) apply (elim conjE)
-  subgoal premises prems for s'
-    proof -
-      have "(execi pre ([], [], ret (Some (type, value))) s) \<rightarrow>\<^sub>i (flowi s (return_value (Some v)))"
-        using prems step_i_step_f.intros register_\<alpha>_eq_dereference
-        by auto
-
-        then show ?thesis using step_deterministic
-          by (metis terminal_impl_no_next_state(1) converse_rtranclpE is_erri_def local.instruction_state.distinct(6)
-              terminal_state_simps(1) prems(2,3,4))
-    qed
-  done
-
-lemma block_ret_None_wp_intro[wp_instrs_intro]:
-  assumes "Q (flowi s (return_value None))"
-  shows "wp_instrs (execi pre ([], [], ret None) s) Q"
-  unfolding wp_instrs_def
-  using assms
-  apply (intro impI allI) apply (elim conjE)
-  subgoal premises prems for s'
-    proof -
-      have "step_i (execi pre ([], [], ret None) s) (flowi s (return_value None))"
-        using prems step_i_step_f.intros
-        by auto
-
-        then show ?thesis using step_deterministic
-          by (metis terminal_impl_no_next_state(1) converse_rtranclpE is_erri_def local.instruction_state.distinct(6)
-              terminal_state_simps(1) prems)
-    qed
-  done
-
-
-lemma block_br_label_wp_intro[wp_instrs_intro]:
-  assumes "Q (flowi s (branch_label l))"
-  shows "wp_instrs (execi pre ([], [], br_label l) s) Q"
-  unfolding wp_instrs_def
-  using assms
-  apply (intro impI allI) apply (elim conjE)
-  by (metis terminal_impl_no_next_state(1) converse_rtranclpE instruction_state.disc(8) local.step_deterministic(1)
-      local.step_i_step_f.intros(1) terminal_state_simps(1))
-
-lemma block_br_i1_wp_intro[wp_instrs_intro]:
-  assumes "register_\<alpha> s value = Some (vi1 b)"
-  assumes "b \<Longrightarrow> Q (flowi s (branch_label l1))"
-  assumes "\<not>b \<Longrightarrow> Q (flowi s (branch_label l2))"
-  shows "wp_instrs (execi pre ([], [], br_i1 value l1 l2) s) Q"
-  unfolding wp_instrs_def
-  using assms
-  apply (intro impI allI) apply (elim conjE)
-  by (smt (verit) terminal_impl_no_next_state converse_rtranclpE instruction_state.collapse(3)
-      instruction_state.distinct(1) local.instruction_state.distinct(6) local.step_deterministic(1) local.step_i.cases
-      local.step_i_step_f.intros(2) register_\<alpha>_eq_dereference)
-
-
-*)
-
-
-
-
-
-
-
-
-
-
-
-
-
-
-
-
-
-
-
+section "Annotations"
 
 type_synonym function_precondition = "state \<Rightarrow> llvm_value list \<Rightarrow> bool"
 type_synonym function_postcondition = "state \<Rightarrow> llvm_value list \<Rightarrow> state \<Rightarrow> llvm_value option \<Rightarrow> bool"
-
 type_synonym block_precondition = "state \<Rightarrow> bool"
 type_synonym block_preconditions = "((llvm_identifier option * llvm_identifier) * block_precondition) list"
-
 type_synonym annotations = "(llvm_identifier * (function_precondition * block_preconditions * function_postcondition)) list"
-
-
 
 context
   fixes annotations :: "annotations"
 begin
 
+
+
+section "Replace Calls"
 
 inductive
   step_i_replaced_calls :: "instruction_state \<Rightarrow> instruction_state \<Rightarrow> bool"
@@ -656,7 +321,6 @@ where
 | "dereference s v = err _ \<Longrightarrow>
     step_i_replaced_calls (execi pre ([],[],ret (Some (t, v))) s) erri"
 
-
 (* Function calls *)
 | "map_of (funcs program) f = Some fu
   \<Longrightarrow> first_label fu = Some b
@@ -671,12 +335,17 @@ where
   \<Longrightarrow> first_label fu = None
   \<Longrightarrow> step_i_replaced_calls (execi pre ([],(call na ty f p)#is,t) s) erri"
 
+(* Precondition Failure / Missing Annotations step to ANY state si' (Chaos Over-approximation) *)
 | "map_of (funcs program) f = Some fu
   \<Longrightarrow> first_label fu = Some b
   \<Longrightarrow> map_of annotations f = Some (fpre,bpres,fpost)
-  \<Longrightarrow> \<not>fpre s []
-  \<Longrightarrow> step_i_replaced_calls (execi pre ([],(call na ty f p)#is,t) s) erri"
+  \<Longrightarrow> \<not>fpre (push_frame s) []
+  \<Longrightarrow> step_i_replaced_calls (execi pre ([],(call na ty f p)#is,t) s) si'"
 
+| "map_of (funcs program) f = Some fu
+  \<Longrightarrow> first_label fu = Some b
+  \<Longrightarrow> map_of annotations f = None
+  \<Longrightarrow> step_i_replaced_calls (execi pre ([],(call na ty f p)#is,t) s) si'"
 
 (* Normal instructions *)
 | "execute_instruction i s = ok s'
@@ -686,24 +355,21 @@ where
   \<Longrightarrow> \<not>is_call i
   \<Longrightarrow> step_i_replaced_calls (execi pre ([],i#is,t) s) erri"
 
-
 (* Phi nodes *)
 | "execute_phi pre p s = ok s' \<Longrightarrow>
     step_i_replaced_calls (execi pre (p#ps,is,t) s) (execi pre (ps,is,t) s')"
 | "execute_phi pre p s = err _ \<Longrightarrow>
     step_i_replaced_calls (execi pre (p#ps,is,t) s) erri"
 
-
 (* Blocks *)
 | "map_of (funcs program) f = Some fu \<Longrightarrow>
     map_of (llvm_function.blocks fu) lab = Some b \<Longrightarrow>
-    step_i_replaced_calls\<^sup>*\<^sup>* (execi prev b s) (flowi s' (branch_label l)) \<Longrightarrow>                                                          
+    step_i_replaced_calls\<^sup>*\<^sup>* (execi prev b s) (flowi s' (branch_label l)) \<Longrightarrow>                                                         
     step_f_replaced_calls (branchf s prev lab f) (branchf s' (Some lab) l f)"
 | "map_of (funcs program) f = Some fu \<Longrightarrow>
     map_of (llvm_function.blocks fu) lab = Some b \<Longrightarrow>
     step_i_replaced_calls\<^sup>*\<^sup>* (execi prev b s) (flowi s' (return_value v)) \<Longrightarrow>
-    step_f_replaced_calls (branchf s prev lab f) (retf s' v)"
-
+    step_f_replaced_calls (branchf s prev lab f) (retf s' v f)"
 
 (* Block errors *)
 | "map_of (funcs program) f = Some fu \<Longrightarrow>
@@ -716,143 +382,229 @@ where
 | "map_of (funcs program) f = None \<Longrightarrow>
      step_f_replaced_calls (branchf s prev lab f) errf"
 
-
-
 definition "wp_func_replaced_calls s p Q \<equiv> \<forall>s'. (step_f_replaced_calls\<^sup>*\<^sup>* s s' \<and> (s' \<nexists>\<rightarrow>\<^sub>f)) \<longrightarrow> wp_steps_f_post s p s' Q"
 
+
 definition "call_verification_condition \<equiv>
-  \<forall>f. map_of (funcs program) f \<noteq> None \<comment> \<open>For all functions in the program\<close>
-    \<longrightarrow> (map_of annotations f \<noteq> None \<comment> \<open>They are annotated\<close>
-    \<and> (\<forall>fpre bpres fpost fu. map_of annotations f = Some (fpre, bpres, fpost) \<and> map_of (funcs program) f = Some fu \<comment> \<open>And for their annotations and the function body\<close>
-      \<longrightarrow> (first_label fu \<noteq> None \<comment> \<open>There is a first block label\<close>
-          \<and> (\<forall>l s. first_label fu = Some l \<and> fpre s [] \<comment> \<open>And for the first block label and all states that satisfy the precondition\<close>
-            \<longrightarrow> wp_func_replaced_calls (branchf s None l f) [] fpost \<comment> \<open>Will satisfy the postcondition of the function with calls replaced\<close>
-            )
-          )
-      )
-    )"
+  ((\<forall>f fu fpre bpres fpost l s.
+    map_of (funcs program) f = Some fu \<and> 
+    map_of annotations f = Some (fpre, bpres, fpost) \<and>
+    first_label fu = Some l \<and> 
+    fpre s []
+    \<longrightarrow> wp_func_replaced_calls (branchf s None l f) [] fpost)
+  \<and> (\<forall>f. map_of (funcs program) f \<noteq> None \<longrightarrow> map_of annotations f \<noteq> None))"
 
-lemma unfolded_wp_vc:
+definition "global_verification_condition \<equiv>
+  ((\<forall>f fu fpre bpres fpost l s.
+    map_of (funcs program) f = Some fu \<and>
+    map_of annotations f = Some (fpre, bpres, fpost) \<and>
+    first_label fu = Some l \<and> 
+    fpre s []
+    \<longrightarrow> wp_steps_f (branchf s None l f) [] fpost)
+  \<and> (\<forall>f. map_of (funcs program) f \<noteq> None \<longrightarrow> map_of annotations f \<noteq> None))"
+
+lemma step_impl_step_replaced:
   assumes "call_verification_condition"
-  assumes "map_of annotations f = Some (fpre, bpres, fpost)"
-  assumes "map_of (funcs program) f = Some fu"
-  assumes "first_label fu = Some l"
-  assumes "fpre s []"
-  assumes "s' \<nexists>\<rightarrow>\<^sub>f"
-  assumes "p = None"
-  assumes "trans_closure_n step_f_n (branchf s p l f) n s'"
-  shows "wp_steps_f_post (branchf s p l f) [] s' fpost"
-proof -
-  have "branchf s None l f \<rightarrow>\<^sub>f* s'"
-    using assms(8) assms(7) n_steps_impl_steps
-    by blast
+  shows "step_i si si' \<Longrightarrow> step_i_replaced_calls si si'"
+    and "step_f sf sf' \<Longrightarrow> step_f_replaced_calls sf sf'"
+proof (induction rule: step_i_step_f.inducts)
+  case (1 pre l s)
+  then show ?case
+    by (simp add: step_i_replaced_calls_step_f_replaced_calls.intros)
+next
+  case (2 s b b' pre l1 l2)
+  then show ?case
+    by (simp add: step_i_replaced_calls_step_f_replaced_calls.intros)
+next
+  case (3 s b pre l1 l2)
+  then show ?case
+    by (simp add: step_i_replaced_calls_step_f_replaced_calls.intros)
+next
+  case (4 pre s)
+  then show ?case
+    by (simp add: step_i_replaced_calls_step_f_replaced_calls.intros)
+next
+  case (5 s v v' pre t)
+  then show ?case
+    by (simp add: step_i_replaced_calls_step_f_replaced_calls.intros)
+next
+  case (6 s v uu pre t)
+  then show ?case
+    by (simp add: step_i_replaced_calls_step_f_replaced_calls.intros)
+next
+  case (7 f fu b s s' v' pre n ty p "is" t)
+ \<comment> \<open> our IH: it holds for the function we call \<close>
+  then have IH_f: "step_f_replaced_calls\<^sup>*\<^sup>* (branchf (push_frame s) None b f) (retf s' v' f)"
+    using mono_rtranclp
+    by (metis (no_types, lifting))
 
-  then show ?thesis
-    using assms(6)
-  proof (induction rule: rtranclp_induct)
-    case base
-    then show ?case
-      by fastforce
-  next
-    case (step smid send)
+  then show ?case
+    \<comment> \<open> depending on if we have annotations\<close>
+    proof (cases "map_of annotations f = None")
+      case True
+      \<comment> \<open> if not - we can step to ANY next state (undeterministic), so that includes the proper state we need \<close>
+      \<comment> \<open> this is safe for our verification since that ALSO means it can step to an error,
+           which means our verification conditions cannot proved if there are no annotations \<close>
+      then show ?thesis
+        by (simp add: "7.IH"(1) "7.hyps" step_i_replaced_calls_step_f_replaced_calls.intros(11))
+    next
+      case False
+      \<comment> \<open> if we have annotations - obtain them \<close>
+      then obtain fpre bpres fpost where annots: "map_of annotations f = Some (fpre, bpres, fpost)"
+        unfolding call_verification_condition_def
+        by fast
 
-    obtain m where "step_f_n smid m send"
-      using step(2) step_impl_exists_n_step
-      by blast
-    then have "m \<le> n"
-      sorry
-
-    obtain ms mp ml mf where "smid = branchf ms mp ml mf"
-      by (metis terminal_impl_no_next_state(2) function_state.collapse(3) function_state.exhaust_disc is_branchf_def is_retf_def step.hyps(2)
-          terminal_state_simps(4,5))
-
-    then show ?case
-      using assms(2,3,4,5,6,7) \<open>m \<le> n\<close>
-    proof (induction n arbitrary: s l f s' rule: less_induct)
-      case (less n s l f s')
-      then show ?case
-      proof (cases "m < n")
+      then show ?thesis
+      \<comment> \<open> depending on if the precondition holds at this point \<close>
+      proof (cases "fpre (push_frame s) []")
         case True
-        
-        then show ?thesis
-          using less
+       \<comment> \<open> the precondition holds, which means the pre/post pair holds (per the verification condition) \<close>
+       then have "wp_func_replaced_calls (branchf (push_frame s) None b f) [] fpost"
+          using assms 7 annots
+          unfolding call_verification_condition_def 
           by blast
+
+       \<comment> \<open> extract the postcondition \<close>
+       hence "wp_steps_f_post (branchf (push_frame s) None b f) [] (retf s' v' f) fpost"
+          unfolding wp_func_replaced_calls_def 
+          using IH_f terminal_f_def by simp
+       hence post_holds: "fpost (push_frame s) [] s' v'"
+          unfolding wp_steps_f_post_def by simp
+
+        \<comment> \<open> and then we have our thesis - we have the postcondition just like in the replaced step relation \<close>
+        then show ?thesis
+          by (simp add: 7 True annots step_i_replaced_calls_step_f_replaced_calls.intros(7))
       next
         case False
-        then have "m = n"
-          using less by force
-
-        then show ?thesis 
-        proof (cases "m = 0")
-          case True
-          then show ?thesis
-            using assms(1)
-            unfolding call_verification_condition_def
-            apply (elim allE[where x=f])
-            apply (elim impE) using less apply blast
-            apply (elim conjE)
-            apply (erule allE[where x=fpre])
-            apply (erule allE[where x=bpres])
-            apply (erule allE[where x=fpost])
-            apply (erule allE[where x=fu])
-            apply (elim impE) using less apply blast
-            apply (elim conjE impE)
-            apply (erule allE[where x=l])
-            apply (erule allE[where x=s])
-            apply (elim impE) using less apply blast
-            unfolding wp_func_replaced_calls_def
-            subgoal premises prems
-          proof -
-            have "step_f_replaced_calls\<^sup>*\<^sup>* smid send"
-              
-              sorry
-            then have "step_f_replaced_calls\<^sup>*\<^sup>* (branchf s p l f) smid"
-              sorry
-            then show ?thesis
-              using less step prems
-              by (metis \<open>local.step_f_replaced_calls\<^sup>*\<^sup>* smid send\<close> rtranclp_trans)
-          qed
-          done
-        next
-          case False
-          then show ?thesis sorry
-        qed
+        \<comment> \<open> if not - we again do not know the next state so we can step to ANY state, safe for the same reason as before \<close>
+        then show ?thesis
+          by (simp add: "7.IH"(1) "7.hyps" annots step_i_replaced_calls_step_f_replaced_calls.intros(10))
       qed
     qed
-  qed
+next
+  case (8 f pre n ty p "is" t s)
+  then show ?case
+    by (simp add: step_i_replaced_calls_step_f_replaced_calls.intros)
+next
+  case (9 f fu pre n ty p "is" t s)
+  then show ?case
+    by (simp add: step_i_replaced_calls_step_f_replaced_calls.intros)
+next
+  case (10 f fu b s pre n ty p "is" t)
+
+  \<comment> \<open> our IH: it holds for the called function \<close>
+  then have IH_f: "step_f_replaced_calls\<^sup>*\<^sup>* (branchf (push_frame s) None b f) errf"
+    using mono_rtranclp
+    by (metis (no_types, lifting))
+
+  then show ?case
+    \<comment> \<open> once again split based on whether we have annotations \<close>
+    proof (cases "map_of annotations f = None")
+      case True
+      \<comment> \<open> if not - we can step to any next state including err \<close>
+      then show ?thesis
+        by (simp add: 10 step_i_replaced_calls_step_f_replaced_calls.intros(11))
+    next
+      case False
+      \<comment> \<open> if we do, obtain them \<close>
+      then obtain fpre bpres fpost where annots: "map_of annotations f = Some (fpre, bpres, fpost)"
+        by fast
+      
+      \<comment> \<open> and show this means we do not satisfy the precondition \<close>
+      then have "\<not> fpre (push_frame s) []"
+      proof -
+        \<comment> \<open> if we did have the precond, then the weakest precondition over steps would hold by our vc  \<close>
+        have "fpre (push_frame s) [] \<Longrightarrow> wp_func_replaced_calls (branchf (push_frame s) None b f) [] fpost"
+          using assms 10 annots
+          unfolding call_verification_condition_def
+          by blast
+        \<comment> \<open> which means it holds for an error \<close>
+        hence "fpre (push_frame s) [] \<Longrightarrow> wp_steps_f_post (branchf (push_frame s) None b f) [] errf fpost"
+          unfolding wp_func_replaced_calls_def 
+          using IH_f terminal_f_def
+          by simp
+        \<comment> \<open> however, that is a contradiction since wp specifies it does not reach errors \<close>
+        then show ?thesis
+          unfolding wp_steps_f_post_def by fastforce
+      qed
+
+      \<comment> \<open> since we don't have the precondition, we can transition to any state including err \<close>
+      then show ?thesis
+        by (simp add: "10.IH"(1) "10.hyps" annots step_i_replaced_calls_step_f_replaced_calls.intros(10))
+    qed
+next
+  case (11 i s s' pre "is" t)
+  then show ?case
+    by (simp add: step_i_replaced_calls_step_f_replaced_calls.intros)
+next
+  case (12 i s uv pre "is" t)
+  then show ?case
+    by (simp add: step_i_replaced_calls_step_f_replaced_calls.intros)
+next
+  case (13 pre p s s' ps "is" t)
+  then show ?case
+    by (simp add: step_i_replaced_calls_step_f_replaced_calls.intros)
+next
+  case (14 pre p s uw ps "is" t)
+  then show ?case
+    by (simp add: step_i_replaced_calls_step_f_replaced_calls.intros)
+next
+  case (15 f fu lab b prev s s' l)
+  then show ?case
+    by (metis (no_types, lifting) mono_rtranclp step_i_replaced_calls_step_f_replaced_calls.intros(16))
+next
+  case (16 f fu lab b prev s s' v)
+  then show ?case
+    by (metis (no_types, lifting) mono_rtranclp step_i_replaced_calls_step_f_replaced_calls.intros(17))
+next
+  case (17 f fu lab b prev s)
+  then show ?case
+    by (metis (no_types, lifting) mono_rtranclp step_i_replaced_calls_step_f_replaced_calls.intros(18))
+next
+  case (18 f fu lab s prev)
+  then show ?case
+    by (simp add: step_i_replaced_calls_step_f_replaced_calls.intros)
+next
+  case (19 f s prev lab)
+  then show ?case
+    by (simp add: step_i_replaced_calls_step_f_replaced_calls.intros)
 qed
 
 
-lemma
-  assumes "call_verification_condition"
-  shows "\<forall>f. map_of (funcs program) f \<noteq> None \<comment> \<open>For all functions in the program\<close>
-    \<longrightarrow> (map_of annotations f \<noteq> None \<comment> \<open>They are annotated\<close>
-    \<and> (\<forall>fpre bpres fpost fu. map_of annotations f = Some (fpre, bpres, fpost) \<and> map_of (funcs program) f = Some fu \<comment> \<open>And for their annotations and the function body\<close>
-      \<longrightarrow> (first_label fu \<noteq> None \<comment> \<open>There is a first block label\<close>
-          \<and> (\<forall>l s. first_label fu = Some l \<and> fpre s [] \<comment> \<open>And for the first block label and all states that satisfy the precondition\<close>
-            \<longrightarrow> wp_steps_f (branchf s None l f) [] fpost \<comment> \<open>Will satisfy the postcondition of the function\<close>
-            )
-          )
-      )
-    )"
-  apply (intro allI impI conjI)
-  subgoal
-    using assms
-    unfolding call_verification_condition_def
-    by blast
-  subgoal
-    using assms
-    unfolding call_verification_condition_def
-    by blast
-  apply simp
-  apply (elim conjE)
-  unfolding wp_steps_f_def
-  apply (intro allI impI)
-  apply (elim conjE)
-  apply (drule steps_impl_exists_n_steps)
-  apply (elim exE)
-  using unfolded_wp_vc assms by blast
 
+
+lemma unfolded_wp_vc:
+  assumes "call_verification_condition"
+  assumes "map_of (funcs program) f = Some fu"
+  assumes "map_of annotations f = Some (fpre, bpres, fpost)"
+  assumes "first_label fu = Some l"
+  assumes "fpre s []"
+  assumes "step_f_replaced_calls\<^sup>*\<^sup>* (branchf s None l f) s'"
+  assumes "s' \<nexists>\<rightarrow>\<^sub>f"
+  shows "wp_steps_f_post (branchf s None l f) [] s' fpost"
+  by (smt (verit, best) Steps.wp_func_replaced_calls_def assms(1,2,3,4,5,6,7) call_verification_condition_def)
+
+
+lemma call_vc_impl_global_vc:
+  "call_verification_condition \<Longrightarrow> global_verification_condition"
+  unfolding global_verification_condition_def wp_steps_f_def
+  apply (intro allI conjI impI)
+   apply (smt (verit, ccfv_threshold) mono_rtranclp step_impl_step_replaced(2) unfolded_wp_vc)
+  unfolding call_verification_condition_def
+  by blast
+
+
+
+section "Floyd Method"
+
+fun replaced_n_steps :: "function_state \<Rightarrow> nat \<Rightarrow> function_state \<Rightarrow> bool" ("_ (\<rightarrow>\<^sub>f\<^sub>R)^_ _" [50,0,51] 50) where
+  "fs \<rightarrow>\<^sub>f\<^sub>R^0 fs' = (fs' = fs)"
+| "fs \<rightarrow>\<^sub>f\<^sub>R^(Suc n) fs' = (\<exists>fs''. step_f_replaced_calls fs fs'' \<and> fs'' \<rightarrow>\<^sub>f\<^sub>R^n fs')"
+
+lemma exists_n_replaced_steps:
+  "step_f_replaced_calls\<^sup>*\<^sup>* fs fs' \<Longrightarrow> \<exists>n. fs \<rightarrow>\<^sub>f\<^sub>R^n fs'"
+  apply (induction rule: converse_rtranclp_induct)
+  using replaced_n_steps.simps by blast+
 
 definition "has_annotation fs \<equiv>
   (case fs of
@@ -861,420 +613,106 @@ definition "has_annotation fs \<equiv>
   | branchf _ p l f \<Rightarrow> map_of (funcs program) f \<noteq> None \<and>
       (case map_of annotations f of 
         None \<Rightarrow> False
-      | Some (fpre,bpres,fpost) \<Rightarrow> map_of bpres (p,l) \<noteq> None
+      | Some (fpre, bpres, fpost) \<Rightarrow> p = None \<or> map_of bpres (p, l) \<noteq> None
       )
   )"
 
-definition "annotation_holds fs \<equiv>
+definition "annotation_holds s_init fs \<equiv>
   (case fs of
     errf \<Rightarrow> False
-  | retf s v f \<Rightarrow> map_of (funcs program) f \<noteq> None \<and>
+  | retf s v f \<Rightarrow> 
       (case map_of annotations f of 
         None \<Rightarrow> False
-      | Some (fpre,bpres,fpost) \<Rightarrow> fpost s v
+      | Some (fpre, bpres, fpost) \<Rightarrow> fpost s_init [] s v
       )
-  | branchf s p l f \<Rightarrow> map_of (funcs program) f \<noteq> None \<and>
+  | branchf s p l f \<Rightarrow> 
       (case map_of annotations f of 
         None \<Rightarrow> False
-      | Some (pres,post) \<Rightarrow>
-          (case map_of pres (p,l) of
-            None \<Rightarrow> False
-          | Some pre \<Rightarrow> pre s
+      | Some (fpre, bpres, fpost) \<Rightarrow>
+          (case p of
+            None \<Rightarrow> fpre s []
+          | Some pred \<Rightarrow> 
+              (case map_of bpres (Some pred, l) of
+                None \<Rightarrow> False
+              | Some pre \<Rightarrow> pre s
+              )
           )
       )
   )"
 
-
 definition step_until :: "function_state \<Rightarrow> function_state \<Rightarrow> bool" where
-  "step_until fs fs' \<equiv> fs \<rightarrow>\<^sub>f fs' \<and> \<not>has_annotation fs"
+  "step_until fs fs' \<equiv> step_f_replaced_calls fs fs' \<and> \<not>has_annotation fs"
 
+definition annotated_step :: "function_state \<Rightarrow> function_state \<Rightarrow> bool" (infix "\<Rightarrow>" 50) where
+  "s \<Rightarrow> s' \<equiv> (\<exists>x. step_f_replaced_calls s x \<and> step_until\<^sup>*\<^sup>* x s') \<and> (has_annotation s' \<or> is_errf s')"
 
-
-definition annotated_step_f :: "function_state \<Rightarrow> function_state \<Rightarrow> bool" (infix "\<Rightarrow>\<^sub>f" 50) where
-  "s \<Rightarrow>\<^sub>f s' \<equiv> (\<exists>x. s \<rightarrow>\<^sub>f x \<and> step_until\<^sup>*\<^sup>* x s') \<and> (has_annotation s' \<or> is_errf s')"
-abbreviation annotated_steps_f :: "function_state \<Rightarrow> function_state \<Rightarrow> bool" (infix "\<Rightarrow>\<^sub>f*" 50) where
-  "fs \<Rightarrow>\<^sub>f* fs' \<equiv> annotated_step_f\<^sup>*\<^sup>* fs fs'"
-
-
+abbreviation annotated_steps :: "function_state \<Rightarrow> function_state \<Rightarrow> bool" (infix "\<Rightarrow>*" 50) where
+  "fs \<Rightarrow>* fs' \<equiv> annotated_step\<^sup>*\<^sup>* fs fs'"
 
 definition wp_step where
-  "wp_step fs Q \<equiv> (\<forall>fs'. fs \<rightarrow>\<^sub>f fs' \<longrightarrow> \<not>is_errf fs' \<and> Q fs')"
+  "wp_step fs Q \<equiv> (\<forall>fs'. step_f_replaced_calls fs fs' \<longrightarrow> \<not>is_errf fs' \<and> Q fs')"
+
+definition wp_func where
+  "wp_func fs Q \<equiv> (\<forall>fs'. fs \<rightarrow>\<^sub>f* fs' \<and> (fs' \<nexists>\<rightarrow>\<^sub>f) \<longrightarrow> \<not>is_errf fs' \<and> (case fs' of retf s' v' _ \<Rightarrow> Q s' v' | _ \<Rightarrow> False))"
+
+definition
+  "wp_func_replaced_calls s Q \<equiv> \<forall>s'. (step_f_replaced_calls\<^sup>*\<^sup>* s s' \<and> (s' \<nexists>\<rightarrow>\<^sub>f)) \<longrightarrow> \<not>is_errf s' \<and> (case s' of retf s_res v_res _ \<Rightarrow> Q s_res v_res | _ \<Rightarrow> False)"
+
+definition "call_verification_condition \<equiv>
+  ((\<forall>f fu pres post l s.
+    map_of (funcs program) f = Some fu \<and> 
+    map_of annotations f = Some (pres, post) \<and>
+    first_label fu = Some l \<and> 
+    (case map_of pres (None, l) of Some precond \<Rightarrow> precond s | None \<Rightarrow> False)
+    \<longrightarrow> wp_func_replaced_calls (branchf s None l f) post)
+  \<and> (\<forall>f. map_of (funcs program) f \<noteq> None \<longrightarrow> map_of annotations f \<noteq> None))"
 
 definition wp_steps_until where
   "wp_steps_until fs Q \<equiv> (\<forall>fs'. (step_until)\<^sup>*\<^sup>* fs fs' \<and> \<not>is_errf fs \<longrightarrow> \<not>is_errf fs') \<and> (\<forall>fs'. (step_until)\<^sup>*\<^sup>* fs fs' \<and> has_annotation fs' \<longrightarrow> Q fs')"
 
 definition wp_annotated_step_f where
-  "wp_annotated_step_f fs Q \<equiv> (\<forall>fs'. fs \<Rightarrow>\<^sub>f fs' \<longrightarrow> \<not>is_errf fs' \<and> Q fs')"
+  "wp_annotated_step_f fs Q \<equiv> (\<forall>fs'. ((fs \<Rightarrow> fs') \<longrightarrow> (\<not>is_errf fs' \<and> Q fs')))"
 
-lemma wp_step_intro:
-  assumes "map_of (funcs program) f = Some fu"
-  assumes "map_of (llvm_function.blocks fu) l = Some b"
-  assumes "wp_instrs
-    (execi p b s)
-    (\<lambda>s'.
-      (case s' of
-        (flowi s'' br) \<Rightarrow>
-          (case br of
-            branch_label l' \<Rightarrow> Q (branchf s'' (Some l) l' f)
-          | return_value v  \<Rightarrow> Q (retf s'' v f)
-          )
-      )
-    )"
-  shows "wp_step (branchf s p l f) Q"
-    using assms
-    unfolding wp_step_def wp_instrs_def
-    apply clarsimp
-    subgoal premises prems for fs'
-    proof (cases fs')
-      case (branchf x11 x12 x13 x14)
-      then show ?thesis
-        by (smt (verit) function_state.disc function_state.sel instruction_state.simps
-            is_errf_def llvm_block_return.simps option.sel prems step_f.cases terminal_state_simps)
-    next
-      case (retf x21 x22)
-      then show ?thesis
-        by (smt (verit) function_state.disc function_state.sel instruction_state.simps
-            is_errf_def llvm_block_return.simps option.sel prems step_f.cases terminal_state_simps)
-    next
-      case errf
-      then show ?thesis
-        by (smt (verit) assms function_state.disc instruction_state.disc function_state.inject function_state.sel instruction_state.simps
-            is_errf_def llvm_block_return.simps option.sel prems step_f.cases terminal_state_simps option.distinct)
-    qed
-    done
-
-lemma wp_steps_until_intro:
-  assumes "has_annotation fs \<Longrightarrow> Q fs"
-  assumes "\<not>has_annotation fs \<Longrightarrow> wp_step  fs (\<lambda>fs'. wp_steps_until fs' Q)"
-  shows "wp_steps_until fs Q"
-  using assms converse_rtranclpE step_until_def
-  unfolding wp_steps_until_def wp_step_def
-  by metis
-
-lemma wp_annotated_step_intro:
-  assumes "wp_step fs (\<lambda>fs'. wp_steps_until fs' Q)"
-  shows "wp_annotated_step_f fs Q"
-  using assms converse_rtranclpE
-  unfolding wp_annotated_step_f_def wp_step_def annotated_step_f_def wp_steps_until_def
-  by blast
-
-
-
-
-
-
-
-
-
-
-lemma instrs_call_intro[wp_instrs_intro]:
-  assumes "map_of (funcs program) f = Some fu"
-  assumes "first_label fu = Some b"
-  assumes "map_of annotations f = Some (pres, post)"
-  assumes "map_of pres (None, b) = Some precond"
-  assumes "precond (push_frame s)"
-  assumes "\<And>s' v'. post s' v' \<Longrightarrow> wp_instrs (execi pre ([], is, t) (pop_frame s s')) Q"
-  shows "wp_instrs (execi pre ([], (call n ty f p)#is, t) s) Q"
-proof -
-  show ?thesis sorry
-qed
-
-
-definition "floyd_cond s p l f \<equiv> wp_annotated_step_f (branchf s p l f) (\<lambda>fs'. annotation_holds fs')"
-
+definition "floyd_cond s_init s p l f \<equiv> wp_annotated_step_f (branchf s p l f) (\<lambda>fs'. annotation_holds s_init fs')"
 
 definition floyd_vc :: "bool" where
   "floyd_vc \<equiv>
-    \<forall>f. map_of (funcs program) f \<noteq> None \<longrightarrow> \<comment> \<open>for all functions in our program\<close>
-    first_label (the (map_of (funcs program) f)) \<noteq> None \<and> \<comment> \<open>there is a first block\<close>
+    \<forall>f. map_of (funcs program) f \<noteq> None \<longrightarrow> 
     (case map_of annotations f of
-      None \<Rightarrow> False \<comment> \<open>and there are annotations\<close>
-    | Some (pres,post) \<Rightarrow>
-        (map_of pres (None, the (first_label (the (map_of (funcs program) f)))) \<noteq> None) \<and> \<comment> \<open>and the first block has a precondition\<close>
-        (\<forall>p l. map_of pres (p,l) \<noteq> None \<longrightarrow> \<comment> \<open>and for all annotated blocks\<close>
-          (\<forall>s. annotation_holds (branchf s p l f) \<longrightarrow> floyd_cond s p l f) \<comment> \<open>all states that satisfy the precond will satisfy any following precond\<close>
+      None \<Rightarrow> False 
+    | Some (fpre, bpres, fpost) \<Rightarrow>
+        (first_label (the (map_of (funcs program) f)) \<noteq> None) \<and> 
+        (\<forall>s_init. fpre s_init [] \<longrightarrow> 
+           floyd_cond s_init s_init None (the (first_label (the (map_of (funcs program) f)))) f) \<and>
+        (\<forall>pred l. map_of bpres (Some pred, l) \<noteq> None \<longrightarrow> 
+           (\<forall>s_init s. annotation_holds s_init (branchf s (Some pred) l f) \<longrightarrow> 
+              floyd_cond s_init s (Some pred) l f)
         )
     )"
 
 
-
-
-
-
-
-
-
-
-
-fun annotation_holds_list where
-  "annotation_holds_list P [] = True"
-| "annotation_holds_list P (((p,l),pre)#pres) = (P p l \<and> annotation_holds_list P pres)"
-
-lemma annotation_holds_list_imp_annotation_holds:
-  assumes "annotation_holds_list (\<lambda>p l. (\<forall>s. annotation_holds (branchf s p l f) \<longrightarrow> floyd_cond s p l f)) pres"
-  shows "(\<forall>p l. map_of pres (p,l) \<noteq> None \<longrightarrow> \<comment> \<open>and for all annotated blocks\<close>
-          (\<forall>s. annotation_holds (branchf s p l f) \<longrightarrow> floyd_cond s p l f) \<comment> \<open>all states that satisfy the precond will satisfy any following precond\<close>
-        )"
+lemma step_until_closure_to_annotated_step:
+  assumes "step_f_replaced_calls fs x"
+  assumes "step_until\<^sup>*\<^sup>* x fs'"
+  assumes "has_annotation fs' \<or> is_errf fs'"
+  shows "fs \<Rightarrow>\<^sub>f fs'"
+  unfolding annotated_step_f_def
   using assms
-  apply (induction pres)
-  apply force
-  subgoal for pre pres
-    apply (intro allI impI)
-    subgoal for p l s
-      apply (cases "pre")
-      subgoal for br precond
-        apply (cases "br = (p,l)")
-        subgoal
-          by (metis (no_types, lifting) annotation_holds_list.simps(2))
-        subgoal premises prems
-        proof -
-          have "annotation_holds_list (\<lambda>p l. (\<forall>s. annotation_holds (branchf s p l f) \<longrightarrow> floyd_cond s p l f)) pres"
-            using prems annotation_holds_list.elims(2)
-            by blast 
-          
-          then show ?thesis
-            using prems map_of_Cons_code(2)
-            by metis
-        qed
-        done
-      done
-    done
-  done
-
-fun annotations_hold_list :: "(llvm_identifier \<Rightarrow> bool) \<Rightarrow> (llvm_identifier * llvm_function) list \<Rightarrow> bool" where
-  "annotations_hold_list P [] = True"
-| "annotations_hold_list P ((fi,fu)#funs) = (P fi \<and> annotations_hold_list P funs)"
-
-lemma annotations_hold_list_imp_floyd_vc:
-  assumes "annotations_hold_list (\<lambda>f. first_label (the (map_of (funcs program) f)) \<noteq> None \<and> \<comment> \<open>there is a first block\<close>
-    (case map_of annotations f of
-      None \<Rightarrow> False \<comment> \<open>and there are annotations\<close>
-    | Some (pres,post) \<Rightarrow>
-        (map_of pres (None, the (first_label (the (map_of (funcs program) f)))) \<noteq> None) \<and> \<comment> \<open>and the first block has a precondition\<close>
-        (\<forall>p l. map_of pres (p,l) \<noteq> None \<longrightarrow> \<comment> \<open>and for all annotated blocks\<close>
-          (\<forall>s. annotation_holds (branchf s p l f) \<longrightarrow> floyd_cond s p l f) \<comment> \<open>all states that satisfy the precond will satisfy any following precond\<close>
-        )
-    )) funs"
-  shows "\<forall>f. map_of (funs) f \<noteq> None \<longrightarrow> \<comment> \<open>for all functions in our program\<close>
-    first_label (the (map_of (funcs program) f)) \<noteq> None \<and> \<comment> \<open>there is a first block\<close>
-    (case map_of annotations f of
-      None \<Rightarrow> False \<comment> \<open>and there are annotations\<close>
-    | Some (pres,post) \<Rightarrow>
-        (map_of pres (None, the (first_label (the (map_of (funcs program) f)))) \<noteq> None) \<and> \<comment> \<open>and the first block has a precondition\<close>
-        (\<forall>p l. map_of pres (p,l) \<noteq> None \<longrightarrow> \<comment> \<open>and for all annotated blocks\<close>
-          (\<forall>s. annotation_holds (branchf s p l f) \<longrightarrow> floyd_cond s p l f) \<comment> \<open>all states that satisfy the precond will satisfy any following precond\<close>
-        )
-    )"
-  using assms
-  apply (induction funs)
-  apply force
-  subgoal for f fs
-    apply (cases f)
-    apply (intro allI impI)
-    subgoal for fi fu f'
-      apply (cases "fi = f'")
-      subgoal
-        using annotations_hold_list.simps(2) n_lists.simps(2) split_cong option.case_eq_if
-        by (smt (verit))
-      subgoal premises prems
-      proof -
-        have "annotations_hold_list (\<lambda>f. first_label (the (map_of (funcs program) f)) \<noteq> None \<and> \<comment> \<open>there is a first block\<close>
-          (case map_of annotations f of
-            None \<Rightarrow> False \<comment> \<open>and there are annotations\<close>
-          | Some (pres,post) \<Rightarrow>
-            (map_of pres (None, the (first_label (the (map_of (funcs program) f)))) \<noteq> None) \<and> \<comment> \<open>and the first block has a precondition\<close>
-              (\<forall>p l. map_of pres (p,l) \<noteq> None \<longrightarrow> \<comment> \<open>and for all annotated blocks\<close>
-                (\<forall>s. annotation_holds (branchf s p l f) \<longrightarrow> floyd_cond s p l f) \<comment> \<open>all states that satisfy the precond will satisfy any following precond\<close>
-              )
-          )) fs" using prems
-          by (metis (no_types, lifting) annotations_hold_list.simps(2))
-        then show ?thesis
-          using prems(1,3,4,5) by fastforce
-      qed
-      done
-    done
-  done
-
-lemma floyd_vc_intro:
-  assumes "annotations_hold_list (\<lambda>f. first_label (the (map_of (funcs program) f)) \<noteq> None \<and> \<comment> \<open>there is a first block\<close>
-    (case map_of annotations f of
-      None \<Rightarrow> False \<comment> \<open>and there are annotations\<close>
-    | Some (pres,post) \<Rightarrow>
-        (map_of pres (None, the (first_label (the (map_of (funcs program) f)))) \<noteq> None) \<and> \<comment> \<open>and the first block has a precondition\<close>
-        (\<forall>p l. map_of pres (p,l) \<noteq> None \<longrightarrow> \<comment> \<open>and for all annotated blocks\<close>
-          (\<forall>s. annotation_holds (branchf s p l f) \<longrightarrow> floyd_cond s p l f) \<comment> \<open>all states that satisfy the precond will satisfy any following precond\<close>
-        )
-    )) (funcs program)"
-  shows "floyd_vc"
-  using assms annotations_hold_list_imp_floyd_vc
-  unfolding floyd_vc_def
   by blast
 
 
-lemma floyd_vc_impl_annotation_holds:
-  assumes "floyd_vc"
-  shows "\<forall>fs fs'. annotation_holds fs \<and> fs \<Rightarrow>\<^sub>f fs' \<longrightarrow> annotation_holds fs'"
-  apply (auto split: function_state.splits)
-  subgoal premises prems for fs fs'
-  proof (cases fs)
-    case (branchf s p l f)
-    then show ?thesis
-      using assms prems
-      unfolding floyd_vc_def floyd_cond_def wp_annotated_step_f_def annotation_holds_def
-      by (smt (verit, ccfv_SIG) case_optionE case_prodE case_prod_conv function_state.simps(9) option.simps(4,5))
-  next
-    case (retf x21 x22 x23)
-    then show ?thesis
-      using annotated_step_f_def local.terminal_state_simps local.terminal_f_def prems
-      by blast
-  next
-    case errf
-    then show ?thesis 
-      using annotated_step_f_def local.terminal_state_simps local.terminal_f_def prems
-      by force 
-  qed
-  done
-
-lemma floyd_vc_impl_annotated_steps_hold:
-  assumes "fs \<Rightarrow>\<^sub>f* fs'"
-  assumes "floyd_vc"
-  assumes "annotation_holds fs"
-  shows "annotation_holds fs'"
-  using assms floyd_vc_impl_annotation_holds
-  by (induction rule: converse_rtranclp_induct; blast)
-
-lemma exists_first_cutpoint:
-  assumes "fs (\<rightarrow>\<^sub>f)^n fs'"
-  assumes "is_errf fs' \<or> has_annotation fs'"
-  shows "\<exists>fsp m. step_until\<^sup>*\<^sup>* fs fsp \<and> (is_errf fsp \<or> has_annotation fsp) \<and> fsp (\<rightarrow>\<^sub>f)^m fs' \<and> m \<le> n"
+lemma steps_impl_annotated_steps:
+  assumes "step_f_replaced_calls\<^sup>*\<^sup>* sf sf'"
+  assumes "has_annotation sf'"
+  shows "sf \<Rightarrow>* sf'"
   using assms
-  proof (induction n arbitrary: fs)
-    case 0
-    
-    then show ?case
-      by force
-  next
-    case (Suc n)
-  
-    then show ?case
-      by (smt (verit, ccfv_threshold) n_steps.elims(1) nat.inject nat_le_linear not_less_eq_eq
-          r_into_rtranclp rtranclp.rtrancl_refl rtranclp_trans step_until_def)
-  qed
-
-
-lemma steps_to_annotation_impl_annotated_steps:
-  assumes path: "fs \<rightarrow>\<^sub>f* fs'"
-  assumes annot: "has_annotation fs' \<or> is_errf fs'"
-  shows "fs \<Rightarrow>\<^sub>f* fs'"
-proof -
-  obtain n where ndef: "fs (\<rightarrow>\<^sub>f)^n fs'" using path closure_steps_exists_n_steps by fast
-  
-  then show ?thesis
-  proof (induction n arbitrary: fs rule: less_induct)
-    case (less n)
-
-    then show ?case
-      proof (cases "n")
-        case 0
-        then show ?thesis
-        using less by fastforce
-      next
-        case (Suc n')
-        then obtain fs1 where fs1def1: "fs \<rightarrow>\<^sub>f fs1" and fs1def: "fs1 (\<rightarrow>\<^sub>f)^n' fs'"
-          using less ndef
-          by auto
-
-        obtain fsa m where "step_until\<^sup>*\<^sup>* fs1 fsa" "has_annotation fsa \<or> is_errf fsa" "fsa (\<rightarrow>\<^sub>f)^m fs'" "m \<le> n'"
-          using fs1def exists_first_cutpoint annot
-          by blast
-
-      then have "fs \<Rightarrow>\<^sub>f fsa" using fs1def1 unfolding annotated_step_f_def by blast
-
-      also from less.IH[OF _ \<open>fsa (\<rightarrow>\<^sub>f)^m fs'\<close>] \<open>m \<le> n'\<close> Suc annot have "fsa \<Rightarrow>\<^sub>f* fs'" by force
-      
-      finally show ?thesis .
-      qed
-    qed
-  qed
-
-
-lemma function_steps_keep_function:
-  assumes "fs \<rightarrow>\<^sub>f* fs'"
-  assumes "fs = branchf s p l f"
-  shows "(case fs' of retf s' v f' \<Rightarrow> f' = f | branchf s' p' l' f' \<Rightarrow> f' = f | errf \<Rightarrow> True)"
-proof (cases fs')
-  case (branchf s' p' l' f')
-  show ?thesis
-    using assms(1)
-    apply (induction rule: rtranclp_induct)
-    using assms(2)
-     apply simp
-    using local.step_f.cases by fastforce
+proof (induction rule: rtranclp_induct)
+  case base
+  then show ?case by simp
 next
-  case (retf x21 x22 x23)
-  show ?thesis 
-    using assms(1)
-    apply (induction rule: rtranclp_induct)
-    using assms(2)
-     apply simp
-    using local.step_f.cases by fastforce
-next
-  case errf
-  then show ?thesis
-    by simp
-qed
-
-
-lemma floyd_vc_impl_wp_step:
-  assumes "floyd_vc"
-  assumes "map_of (funcs program) f = Some fu"
-  assumes "map_of annotations f = Some (pres,post)"
-  assumes "first_label fu = Some fl"
-  assumes "annotation_holds fs"
-  assumes "fs = branchf s None fl f"
-  shows "wp_func fs post"
-  unfolding wp_func_def
-  apply (intro allI impI)
-  subgoal premises prems for fs'
-  proof -
-    have "has_annotation fs'"
-      unfolding has_annotation_def 
-      by (smt (verit, ccfv_SIG) Steps.terminal_non_err annotation_holds_def assms(1,5) floyd_vc_def
-          floyd_vc_impl_annotated_steps_hold function_state.case_eq_if function_state.disc(2) function_state.sel(7)
-          function_state.simps(11) function_state.split_sel_asm is_errf_def le_boolD local.step_f.cases
-          local.terminal_state_simps(3) option.distinct(1) option.simps(4) prems rtranclp.simps
-          steps_to_annotation_impl_annotated_steps)
-    
-    then have "fs \<Rightarrow>\<^sub>f* fs'" using prems steps_to_annotation_impl_annotated_steps
-      by blast
-
-    then have "annotation_holds fs'"
-      using assms(1,5) floyd_vc_impl_annotated_steps_hold by blast
-
-    then show ?thesis
-      using prems
-      unfolding annotation_holds_def
-      apply (cases fs')
-      defer defer apply force defer apply (erule conjE)
-      subgoal premises prems' for s v f'
-      proof -
-        have "f = f'" using prems' function_steps_keep_function assms function_state.simps
-          by (smt (verit, ccfv_threshold))
-
-        then show ?thesis
-          using assms prems'
-          by force
-      qed
-      
-      done
-  qed
-  done
-
-end
+  case (step y z)
+  from step.IH show ?case
 
 
 end
-
-
-
 end
